A few more stages fixed up

09HeapMemory/HeapConversion.thy
@@ -14,18 +14,20 @@ reference values that haven't even been allocated yet.\<close>
 fun unheap_closure :: "closure\<^sub>h heap \<Rightarrow> ptr \<Rightarrow> closure\<^sub>b" where
   "unheap_closure h x = (case hlookup h x of 
       Const\<^sub>h n \<Rightarrow> Const\<^sub>b n
-    | Lam\<^sub>h \<Delta> p \<Rightarrow> Lam\<^sub>b (if list_all ((>) x) \<Delta> then map (unheap_closure h) \<Delta> else undefined) p)"
+    | Lam\<^sub>h \<Delta> p n \<Rightarrow> Lam\<^sub>b (if list_all (list_all ((>) x)) \<Delta> then map (map (unheap_closure h)) \<Delta> 
+        else undefined) p n)"
 
-abbreviation unheap_stack :: "closure\<^sub>h heap \<Rightarrow> (ptr list \<times> nat) list \<Rightarrow> (closure\<^sub>b list \<times> nat) list" 
-    where
-  "unheap_stack h s \<equiv> map (\<lambda>(\<Delta>, p). (map (unheap_closure h) \<Delta>, p)) s"
+abbreviation unheap_stack :: "closure\<^sub>h heap \<Rightarrow> (ptr list list \<times> nat) list \<Rightarrow> 
+    (closure\<^sub>b list list \<times> nat) list" where
+  "unheap_stack h s \<equiv> map (\<lambda>(\<Delta>, p). (map (map (unheap_closure h)) \<Delta>, p)) s"
 
 primrec unheap :: "state\<^sub>h \<Rightarrow> state\<^sub>b" where
   "unheap (S\<^sub>h h \<V> s) = S\<^sub>b (map (unheap_closure h) \<V>) (unheap_stack h s)"
 
 primrec bounded_closure :: "closure\<^sub>h heap \<Rightarrow> ptr \<Rightarrow> closure\<^sub>h \<Rightarrow> bool" where
   "bounded_closure h x (Const\<^sub>h n) = True"
-| "bounded_closure h x (Lam\<^sub>h \<Delta> p) = (list_all (hcontains h) \<Delta> \<and> list_all ((>) x) \<Delta>)"
+| "bounded_closure h x (Lam\<^sub>h \<Delta> p n) = 
+    (list_all (list_all (hcontains h)) \<Delta> \<and> list_all (list_all ((>) x)) \<Delta>)"
 
 lemma halloc_bounded [simp]: "halloc h a = (h', x) \<Longrightarrow> bounded_closure h y c \<Longrightarrow> 
     bounded_closure h' y c"
@@ -48,11 +50,12 @@ proof (induction h x rule: unheap_closure.induct)
   proof (cases "hlookup h x")
     case (Lam\<^sub>h \<Delta> p)
     with 1 show ?thesis
-    proof (cases "list_all ((>) x) \<Delta>")
+    proof (cases "list_all (list_all ((>) x)) \<Delta>")
       case True
-      from Lam\<^sub>h 1 have "list_all (hcontains h) \<Delta>" by (metisx hlookup_all bounded_closure.simps(2))
-      hence S: "\<And>y. y \<in> set \<Delta> \<Longrightarrow> hcontains h y" by auto
-      from 1 Lam\<^sub>h True have "\<And>y. y \<in> set \<Delta> \<Longrightarrow> hcontains h y \<Longrightarrow> 
+      from Lam\<^sub>h 1 have "list_all (list_all (hcontains h)) \<Delta>" 
+        by (metis hlookup_all bounded_closure.simps(2))
+      hence S: "\<And>vs y. vs \<in> set \<Delta> \<Longrightarrow> y \<in> set vs \<Longrightarrow> hcontains h y" by auto
+      from 1 Lam\<^sub>h True have "\<And>y vs. vs \<in> set \<Delta> \<Longrightarrow> y \<in> set vs \<Longrightarrow> hcontains h y \<Longrightarrow> 
         unheap_closure h' y = unheap_closure h y" by simp
       with S 1(2, 3) Lam\<^sub>h True show ?thesis by simp
     qed simp_all
@@ -63,29 +66,34 @@ lemma halloc_unheap_env [simp]: "halloc h c = (h', v) \<Longrightarrow> list_all
     heap_all (bounded_closure h) h \<Longrightarrow> map (unheap_closure h') \<Delta> = map (unheap_closure h) \<Delta>"
   by (induction \<Delta>) (simp_all del: unheap_closure.simps)
 
+lemma halloc_unheap_list_env [simp]: "halloc h c = (h', v) \<Longrightarrow> 
+  list_all (list_all (hcontains h)) \<Delta> \<Longrightarrow> heap_all (bounded_closure h) h \<Longrightarrow> 
+    map (map (unheap_closure h')) \<Delta> = map (map (unheap_closure h)) \<Delta>"
+  by (induction \<Delta>) (simp_all del: unheap_closure.simps)
+
 lemma halloc_unheap_stack [simp]: "halloc h c = (h', v) \<Longrightarrow> 
-  list_all (list_all (hcontains h)) (map fst s) \<Longrightarrow> heap_all (bounded_closure h) h \<Longrightarrow> 
+  list_all (list_all (list_all (hcontains h))) (map fst s) \<Longrightarrow> heap_all (bounded_closure h) h \<Longrightarrow> 
     unheap_stack h' s = unheap_stack h s"
   by (induction s) (auto simp del: unheap_closure.simps)
 
-lemma hlookup_lam_bounded [simp]: "hlookup h v = Lam\<^sub>h \<Delta> p \<Longrightarrow> heap_all (bounded_closure h) h \<Longrightarrow> 
-    hcontains h v \<Longrightarrow> list_all ((>) v) \<Delta>"
+lemma hlookup_lam_bounded [simp]: "hlookup h v = Lam\<^sub>h \<Delta> p n \<Longrightarrow> heap_all (bounded_closure h) h \<Longrightarrow> 
+    hcontains h v \<Longrightarrow> list_all (list_all ((>) v)) \<Delta>"
   by (metis hlookup_all bounded_closure.simps(2))
 
 primrec heap_structured :: "state\<^sub>h \<Rightarrow> bool" where
   "heap_structured (S\<^sub>h h \<V> s) = (heap_all (bounded_closure h) h \<and>
-    list_all (hcontains h) \<V> \<and> list_all (list_all (hcontains h)) (map fst s))"
+    list_all (hcontains h) \<V> \<and> list_all (list_all (list_all (hcontains h))) (map fst s))"
 
 lemma eval_heap_structured [simp]: "\<C> \<tturnstile> \<Sigma>\<^sub>h \<leadsto>\<^sub>h \<Sigma>\<^sub>h' \<Longrightarrow> heap_structured \<Sigma>\<^sub>h \<Longrightarrow> heap_structured \<Sigma>\<^sub>h'"
 proof (induction \<Sigma>\<^sub>h \<Sigma>\<^sub>h' rule: eval\<^sub>h.induct)
-  case (ev\<^sub>h_apply \<C> p h v\<^sub>2 \<Delta> p' v\<^sub>1 \<V> s)
-  hence "hlookup h v\<^sub>2 = Lam\<^sub>h \<Delta> p' \<and> heap_all (bounded_closure h) h \<and> hcontains h v\<^sub>2" by simp
-  hence "bounded_closure h v\<^sub>2 (Lam\<^sub>h \<Delta> p')" by (metis hlookup_all)
+  case (ev\<^sub>h_apply \<C> p h v\<^sub>2 \<Delta> p' n v\<^sub>1 \<V> s)
+  hence "hlookup h v\<^sub>2 = Lam\<^sub>h \<Delta> p' n \<and> heap_all (bounded_closure h) h \<and> hcontains h v\<^sub>2" by simp
+  hence "bounded_closure h v\<^sub>2 (Lam\<^sub>h \<Delta> p' n)" by (metis hlookup_all)
   with ev\<^sub>h_apply show ?case by simp
 next
-  case (ev\<^sub>h_jump \<C> p h v\<^sub>2 \<Delta>' p' v\<^sub>1 \<V> \<Delta> s)
-  hence "hlookup h v\<^sub>2 = Lam\<^sub>h \<Delta>' p' \<and> heap_all (bounded_closure h) h \<and> hcontains h v\<^sub>2" by simp
-  hence "bounded_closure h v\<^sub>2 (Lam\<^sub>h \<Delta>' p')" by (metis hlookup_all)
+  case (ev\<^sub>h_jump \<C> p h v\<^sub>2 \<Delta>' p' n v\<^sub>1 \<V> \<Delta> s)
+  hence "hlookup h v\<^sub>2 = Lam\<^sub>h \<Delta>' p' n \<and> heap_all (bounded_closure h) h \<and> hcontains h v\<^sub>2" by simp
+  hence "bounded_closure h v\<^sub>2 (Lam\<^sub>h \<Delta>' p' n)" by (metis hlookup_all)
   with ev\<^sub>h_jump show ?case by simp
 qed fastforce+
 
@@ -105,32 +113,32 @@ qed
 
 lemma unheap_to_cons [simp]: "S\<^sub>b \<V>\<^sub>b ((\<Delta>, p) # s) = unheap \<Sigma>\<^sub>h \<Longrightarrow> \<exists>h \<V>\<^sub>h \<Delta>\<^sub>h s\<^sub>h. 
   \<Sigma>\<^sub>h = S\<^sub>h h \<V>\<^sub>h ((\<Delta>\<^sub>h, p) # s\<^sub>h) \<and> \<V>\<^sub>b = map (unheap_closure h) \<V>\<^sub>h \<and> 
-    \<Delta> = map (unheap_closure h) \<Delta>\<^sub>h \<and> s = unheap_stack h s\<^sub>h"
+    \<Delta> = map (map (unheap_closure h)) \<Delta>\<^sub>h \<and> s = unheap_stack h s\<^sub>h"
 proof (induction \<Sigma>\<^sub>h)
   case (S\<^sub>h h \<V>\<^sub>h s\<^sub>h)
   thus ?case by (induction s\<^sub>h) (auto simp del: unheap_closure.simps)
 qed 
 
-lemma unheap_to_lam [simp]: "unheap_closure h v = Lam\<^sub>b \<Delta>\<^sub>b p \<Longrightarrow> hcontains h v \<Longrightarrow> 
+lemma unheap_to_lam [simp]: "unheap_closure h v = Lam\<^sub>b \<Delta>\<^sub>b p n \<Longrightarrow> hcontains h v \<Longrightarrow> 
   heap_all (bounded_closure h) h \<Longrightarrow> 
-    \<exists>\<Delta>\<^sub>h. hlookup h v = Lam\<^sub>h \<Delta>\<^sub>h p \<and> \<Delta>\<^sub>b = map (unheap_closure h) \<Delta>\<^sub>h"
+    \<exists>\<Delta>\<^sub>h. hlookup h v = Lam\<^sub>h \<Delta>\<^sub>h p n \<and> \<Delta>\<^sub>b = map (map (unheap_closure h)) \<Delta>\<^sub>h"
   by (simp split: closure\<^sub>h.splits if_splits)
 
 theorem correct\<^sub>h [simp]: "\<C> \<tturnstile> unheap \<Sigma>\<^sub>h \<leadsto>\<^sub>b \<Sigma>\<^sub>b' \<Longrightarrow> heap_structured \<Sigma>\<^sub>h \<Longrightarrow> 
   \<exists>\<Sigma>\<^sub>h'. (\<C> \<tturnstile> \<Sigma>\<^sub>h \<leadsto>\<^sub>h \<Sigma>\<^sub>h') \<and> \<Sigma>\<^sub>b' = unheap \<Sigma>\<^sub>h'"
 proof (induction "unheap \<Sigma>\<^sub>h" \<Sigma>\<^sub>b' rule: eval\<^sub>b.induct)
-  case (ev\<^sub>b_lookup \<C> p x y z \<Delta>\<^sub>b v \<V>\<^sub>b s\<^sub>b)
+  case (ev\<^sub>b_lookup \<C> p x y \<Delta>\<^sub>b vs v \<V>\<^sub>b s\<^sub>b)
   then obtain h \<V>\<^sub>h \<Delta>\<^sub>h s\<^sub>h where "\<Sigma>\<^sub>h = S\<^sub>h h \<V>\<^sub>h ((\<Delta>\<^sub>h, Suc p) # s\<^sub>h) \<and> \<V>\<^sub>b = map (unheap_closure h) \<V>\<^sub>h \<and> 
-    \<Delta>\<^sub>b = map (unheap_closure h) \<Delta>\<^sub>h \<and> s\<^sub>b = unheap_stack h s\<^sub>h" by fastforce
-  moreover with ev\<^sub>b_lookup obtain vv where "lookup \<Delta>\<^sub>h x = Some vv \<and> v = unheap_closure h vv" 
-    by fastforce
-  moreover with ev\<^sub>b_lookup have "\<C> \<tturnstile> S\<^sub>h h \<V>\<^sub>h ((\<Delta>\<^sub>h, Suc p) # s\<^sub>h) \<leadsto>\<^sub>h S\<^sub>h h (vv # \<V>\<^sub>h) ((\<Delta>\<^sub>h, p) # s\<^sub>h)" 
+    \<Delta>\<^sub>b = map (map (unheap_closure h)) \<Delta>\<^sub>h \<and> s\<^sub>b = unheap_stack h s\<^sub>h" by fastforce
+  moreover with ev\<^sub>b_lookup obtain vs' v' where "lookup \<Delta>\<^sub>h x = Some vs' \<and> lookup vs' y = Some v' \<and> 
+    v = unheap_closure h v'" by fastforce
+  moreover with ev\<^sub>b_lookup have "\<C> \<tturnstile> S\<^sub>h h \<V>\<^sub>h ((\<Delta>\<^sub>h, Suc p) # s\<^sub>h) \<leadsto>\<^sub>h S\<^sub>h h (v' # \<V>\<^sub>h) ((\<Delta>\<^sub>h, p) # s\<^sub>h)" 
     by simp
   ultimately show ?case by fastforce
 next
   case (ev\<^sub>b_pushcon \<C> p n \<V>\<^sub>b \<Delta>\<^sub>b s\<^sub>b)
   moreover then obtain h \<V>\<^sub>h \<Delta>\<^sub>h s\<^sub>h where "\<Sigma>\<^sub>h = S\<^sub>h h \<V>\<^sub>h ((\<Delta>\<^sub>h, Suc p) # s\<^sub>h) \<and> 
-    \<V>\<^sub>b = map (unheap_closure h) \<V>\<^sub>h \<and> \<Delta>\<^sub>b = map (unheap_closure h) \<Delta>\<^sub>h \<and> s\<^sub>b = unheap_stack h s\<^sub>h" 
+    \<V>\<^sub>b = map (unheap_closure h) \<V>\<^sub>h \<and> \<Delta>\<^sub>b = map (map (unheap_closure h)) \<Delta>\<^sub>h \<and> s\<^sub>b = unheap_stack h s\<^sub>h" 
       by fastforce
   moreover obtain h' v where "halloc h (Const\<^sub>h n) = (h', v)" by fastforce
   moreover with ev\<^sub>b_pushcon have "\<C> \<tturnstile> S\<^sub>h h \<V>\<^sub>h ((\<Delta>\<^sub>h, Suc p) # s\<^sub>h) \<leadsto>\<^sub>h S\<^sub>h h' (v # \<V>\<^sub>h) ((\<Delta>\<^sub>h, p) # s\<^sub>h)" 
@@ -139,51 +147,51 @@ next
 next
   case (ev\<^sub>b_pushlam \<C> p p' n \<V>\<^sub>b \<Delta>\<^sub>b s\<^sub>b)
   moreover then obtain h \<V>\<^sub>h \<Delta>\<^sub>h s\<^sub>h where S: "\<Sigma>\<^sub>h = S\<^sub>h h \<V>\<^sub>h ((\<Delta>\<^sub>h, Suc p) # s\<^sub>h) \<and> 
-    \<V>\<^sub>b = map (unheap_closure h) \<V>\<^sub>h \<and> \<Delta>\<^sub>b = map (unheap_closure h) \<Delta>\<^sub>h \<and> s\<^sub>b = unheap_stack h s\<^sub>h" 
+    \<V>\<^sub>b = map (unheap_closure h) \<V>\<^sub>h \<and> \<Delta>\<^sub>b = map (map (unheap_closure h)) \<Delta>\<^sub>h \<and> s\<^sub>b = unheap_stack h s\<^sub>h" 
       by fastforce
-  moreover obtain h' v where "halloc h (Lam\<^sub>h \<Delta>\<^sub>h p') = (h', v)" by fastforce
+  moreover obtain h' v where "halloc h (Lam\<^sub>h \<Delta>\<^sub>h p' n) = (h', v)" by fastforce
   moreover with ev\<^sub>b_pushlam S have "\<C> \<tturnstile> S\<^sub>h h \<V>\<^sub>h ((\<Delta>\<^sub>h, Suc p) # s\<^sub>h) \<leadsto>\<^sub>h S\<^sub>h h' (v # \<V>\<^sub>h) ((\<Delta>\<^sub>h, p) # s\<^sub>h)" 
     by simp
   ultimately show ?case by fastforce
 next
-  case (ev\<^sub>b_apply \<C> p v\<^sub>b \<Delta>\<^sub>b' p' \<V>\<^sub>b \<Delta>\<^sub>b s\<^sub>b)
+  case (ev\<^sub>b_apply \<C> p v\<^sub>b \<Delta>\<^sub>b' p' n \<V>\<^sub>b \<Delta>\<^sub>b s\<^sub>b)
   then obtain h \<V>\<^sub>h' \<Delta>\<^sub>h s\<^sub>h where S: "\<Sigma>\<^sub>h = S\<^sub>h h \<V>\<^sub>h' ((\<Delta>\<^sub>h, Suc p) # s\<^sub>h) \<and> 
-    v\<^sub>b # Lam\<^sub>b \<Delta>\<^sub>b' p' # \<V>\<^sub>b = map (unheap_closure h) \<V>\<^sub>h' \<and> \<Delta>\<^sub>b = map (unheap_closure h) \<Delta>\<^sub>h \<and> 
+    v\<^sub>b # Lam\<^sub>b \<Delta>\<^sub>b' p' n # \<V>\<^sub>b = map (unheap_closure h) \<V>\<^sub>h' \<and> \<Delta>\<^sub>b = map (map (unheap_closure h)) \<Delta>\<^sub>h \<and> 
       s\<^sub>b = unheap_stack h s\<^sub>h" by fastforce
   moreover then obtain v\<^sub>h\<^sub>1 v\<^sub>h\<^sub>2 \<V>\<^sub>h where "\<V>\<^sub>h' = v\<^sub>h\<^sub>1 # v\<^sub>h\<^sub>2 # \<V>\<^sub>h \<and> v\<^sub>b = unheap_closure h v\<^sub>h\<^sub>1 \<and> 
-    Lam\<^sub>b \<Delta>\<^sub>b' p' = unheap_closure h v\<^sub>h\<^sub>2 \<and> \<V>\<^sub>b = map (unheap_closure h) \<V>\<^sub>h" by fastforce
-  moreover with ev\<^sub>b_apply S obtain \<Delta>h' where H: "hlookup h v\<^sub>h\<^sub>2 = Lam\<^sub>h \<Delta>h' p' \<and> 
-    \<Delta>\<^sub>b' = map (unheap_closure h) \<Delta>h'" by fastforce
+    Lam\<^sub>b \<Delta>\<^sub>b' p' n = unheap_closure h v\<^sub>h\<^sub>2 \<and> \<V>\<^sub>b = map (unheap_closure h) \<V>\<^sub>h" by fastforce
+  moreover with ev\<^sub>b_apply S obtain \<Delta>h' where H: "hlookup h v\<^sub>h\<^sub>2 = Lam\<^sub>h \<Delta>h' p' n \<and> 
+    \<Delta>\<^sub>b' = map (map (unheap_closure h)) \<Delta>h'" by fastforce
   moreover with ev\<^sub>b_apply have "\<C> \<tturnstile> S\<^sub>h h (v\<^sub>h\<^sub>1 # v\<^sub>h\<^sub>2 # \<V>\<^sub>h) ((\<Delta>\<^sub>h, Suc p) # s\<^sub>h) \<leadsto>\<^sub>h 
-    S\<^sub>h h \<V>\<^sub>h ((v\<^sub>h\<^sub>1 # \<Delta>h', p') # (\<Delta>\<^sub>h, p) # s\<^sub>h)" by simp
+    S\<^sub>h h \<V>\<^sub>h (([v\<^sub>h\<^sub>1] # \<Delta>h', p') # (\<Delta>\<^sub>h, p) # s\<^sub>h)" by simp
   ultimately show ?case by fastforce
 next
   case (ev\<^sub>b_pushenv \<C> p v\<^sub>b \<V>\<^sub>b \<Delta>\<^sub>b s\<^sub>b)
   then obtain h \<V>\<^sub>h' \<Delta>\<^sub>h s\<^sub>h where "\<Sigma>\<^sub>h = S\<^sub>h h \<V>\<^sub>h' ((\<Delta>\<^sub>h, Suc p) # s\<^sub>h) \<and> 
-    v\<^sub>b # \<V>\<^sub>b = map (unheap_closure h) \<V>\<^sub>h' \<and> \<Delta>\<^sub>b = map (unheap_closure h) \<Delta>\<^sub>h \<and> s\<^sub>b = unheap_stack h s\<^sub>h" 
-      by fastforce
+    v\<^sub>b # \<V>\<^sub>b = map (unheap_closure h) \<V>\<^sub>h' \<and> \<Delta>\<^sub>b = map (map (unheap_closure h)) \<Delta>\<^sub>h \<and> 
+      s\<^sub>b = unheap_stack h s\<^sub>h" by fastforce
   moreover then obtain v\<^sub>h \<V>\<^sub>h where "\<V>\<^sub>h' = v\<^sub>h # \<V>\<^sub>h \<and> v\<^sub>b = unheap_closure h v\<^sub>h \<and> 
     \<V>\<^sub>b = map (unheap_closure h) \<V>\<^sub>h" by fastforce
   moreover from ev\<^sub>b_pushenv have "\<C> \<tturnstile> S\<^sub>h h (v\<^sub>h # \<V>\<^sub>h) ((\<Delta>\<^sub>h, Suc p) # s\<^sub>h) \<leadsto>\<^sub>h 
-    S\<^sub>h h \<V>\<^sub>h ((v\<^sub>h # \<Delta>\<^sub>h, p) # s\<^sub>h)" by simp
+    S\<^sub>h h \<V>\<^sub>h ((cons_fst v\<^sub>h \<Delta>\<^sub>h, p) # s\<^sub>h)" by simp
   ultimately show ?case by fastforce
 next
   case (ev\<^sub>b_return \<C> p \<V>\<^sub>b \<Delta>\<^sub>b s\<^sub>b)
   then obtain h \<V>\<^sub>h \<Delta>\<^sub>h s\<^sub>h where "\<Sigma>\<^sub>h = S\<^sub>h h \<V>\<^sub>h ((\<Delta>\<^sub>h, Suc p) # s\<^sub>h) \<and> \<V>\<^sub>b = map (unheap_closure h) \<V>\<^sub>h \<and> 
-    \<Delta>\<^sub>b = map (unheap_closure h) \<Delta>\<^sub>h \<and> s\<^sub>b = unheap_stack h s\<^sub>h" by fastforce
+    \<Delta>\<^sub>b = map (map (unheap_closure h)) \<Delta>\<^sub>h \<and> s\<^sub>b = unheap_stack h s\<^sub>h" by fastforce
   moreover with ev\<^sub>b_return have "\<C> \<tturnstile> S\<^sub>h h \<V>\<^sub>h ((\<Delta>\<^sub>h, Suc p) # s\<^sub>h) \<leadsto>\<^sub>h S\<^sub>h h \<V>\<^sub>h s\<^sub>h" by simp
   ultimately show ?case by fastforce
 next
-  case (ev\<^sub>b_jump \<C> p v\<^sub>b \<Delta>\<^sub>b' p' \<V>\<^sub>b \<Delta>\<^sub>b s\<^sub>b)
+  case (ev\<^sub>b_jump \<C> p v\<^sub>b \<Delta>\<^sub>b' p' n \<V>\<^sub>b \<Delta>\<^sub>b s\<^sub>b)
   then obtain h \<V>\<^sub>h' \<Delta>\<^sub>h s\<^sub>h where S: "\<Sigma>\<^sub>h = S\<^sub>h h \<V>\<^sub>h' ((\<Delta>\<^sub>h, Suc p) # s\<^sub>h) \<and> 
-    v\<^sub>b # Lam\<^sub>b \<Delta>\<^sub>b' p' # \<V>\<^sub>b = map (unheap_closure h) \<V>\<^sub>h' \<and> \<Delta>\<^sub>b = map (unheap_closure h) \<Delta>\<^sub>h \<and> 
+    v\<^sub>b # Lam\<^sub>b \<Delta>\<^sub>b' p' n # \<V>\<^sub>b = map (unheap_closure h) \<V>\<^sub>h' \<and> \<Delta>\<^sub>b = map (map (unheap_closure h)) \<Delta>\<^sub>h \<and> 
       s\<^sub>b = unheap_stack h s\<^sub>h" by fastforce
   moreover from S obtain v\<^sub>h\<^sub>1 v\<^sub>h\<^sub>2 \<V>\<^sub>h where "\<V>\<^sub>h' = v\<^sub>h\<^sub>1 # v\<^sub>h\<^sub>2 # \<V>\<^sub>h \<and> v\<^sub>b = unheap_closure h v\<^sub>h\<^sub>1 \<and> 
-    Lam\<^sub>b \<Delta>\<^sub>b' p' = unheap_closure h v\<^sub>h\<^sub>2 \<and> \<V>\<^sub>b = map (unheap_closure h) \<V>\<^sub>h" by fastforce
-  moreover with ev\<^sub>b_jump S obtain \<Delta>h' where "hlookup h v\<^sub>h\<^sub>2 = Lam\<^sub>h \<Delta>h' p' \<and> 
-    \<Delta>\<^sub>b' = map (unheap_closure h) \<Delta>h'" by fastforce
+    Lam\<^sub>b \<Delta>\<^sub>b' p' n = unheap_closure h v\<^sub>h\<^sub>2 \<and> \<V>\<^sub>b = map (unheap_closure h) \<V>\<^sub>h" by fastforce
+  moreover with ev\<^sub>b_jump S obtain \<Delta>h' where "hlookup h v\<^sub>h\<^sub>2 = Lam\<^sub>h \<Delta>h' p' n \<and> 
+    \<Delta>\<^sub>b' = map (map (unheap_closure h)) \<Delta>h'" by fastforce
   moreover with ev\<^sub>b_jump S have "\<C> \<tturnstile> S\<^sub>h h (v\<^sub>h\<^sub>1 # v\<^sub>h\<^sub>2 # \<V>\<^sub>h) ((\<Delta>\<^sub>h, Suc p) # s\<^sub>h) \<leadsto>\<^sub>h 
-    S\<^sub>h h \<V>\<^sub>h ((v\<^sub>h\<^sub>1 # \<Delta>h', p') # s\<^sub>h)" by simp
+    S\<^sub>h h \<V>\<^sub>h (([v\<^sub>h\<^sub>1] # \<Delta>h', p') # s\<^sub>h)" by simp
   ultimately show ?case by fastforce
 qed
 
