09HeapMemory/HeapMemory.thy
@@ -12,35 +12,36 @@ now.\<close>
 
 datatype closure\<^sub>h = 
   Const\<^sub>h nat
-  | Lam\<^sub>h "ptr list" nat
+  | Lam\<^sub>h "ptr list list" nat nat
 
 datatype state\<^sub>h = 
-  S\<^sub>h "closure\<^sub>h heap" "ptr list" "(ptr list \<times> nat) list"
+  S\<^sub>h "closure\<^sub>h heap" "ptr list" "(ptr list list \<times> nat) list"
 
 text \<open>Our evaluation relation must now \<open>halloc\<close> values when pushing them, and \<open>hlookup\<close> them when 
 popping; but beyond that, things are mostly the same as the previous stage, and we no longer 
 duplicate values, only pointers to them.\<close>
 
 inductive eval\<^sub>h :: "code\<^sub>b list \<Rightarrow> state\<^sub>h \<Rightarrow> state\<^sub>h \<Rightarrow> bool" (infix "\<tturnstile> _ \<leadsto>\<^sub>h" 50) where
-  ev\<^sub>h_lookup [simp]: "lookup \<C> p = Some (Lookup\<^sub>b x y z) \<Longrightarrow> lookup \<Delta> x = Some v \<Longrightarrow> 
-    \<C> \<tturnstile> S\<^sub>h h \<V> ((\<Delta>, Suc p) # s) \<leadsto>\<^sub>h S\<^sub>h h (v # \<V>) ((\<Delta>, p) # s)"
+  ev\<^sub>h_lookup [simp]: "lookup \<C> p = Some (Lookup\<^sub>b x y) \<Longrightarrow> lookup \<Delta> x = Some vs \<Longrightarrow> 
+    lookup vs y = Some v \<Longrightarrow>
+      \<C> \<tturnstile> S\<^sub>h h \<V> ((\<Delta>, Suc p) # s) \<leadsto>\<^sub>h S\<^sub>h h (v # \<V>) ((\<Delta>, p) # s)"
 | ev\<^sub>h_pushcon [simp]: "lookup \<C> p = Some (PushCon\<^sub>b n) \<Longrightarrow> halloc h (Const\<^sub>h n) = (h', v) \<Longrightarrow>
     \<C> \<tturnstile> S\<^sub>h h \<V> ((\<Delta>, Suc p) # s) \<leadsto>\<^sub>h S\<^sub>h h' (v # \<V>) ((\<Delta>, p) # s)"
-| ev\<^sub>h_pushlam [simp]: "lookup \<C> p = Some (PushLam\<^sub>b p' n) \<Longrightarrow> halloc h (Lam\<^sub>h \<Delta> p') = (h', v) \<Longrightarrow>
+| ev\<^sub>h_pushlam [simp]: "lookup \<C> p = Some (PushLam\<^sub>b p' n) \<Longrightarrow> halloc h (Lam\<^sub>h \<Delta> p' n) = (h', v) \<Longrightarrow>
     \<C> \<tturnstile> S\<^sub>h h \<V> ((\<Delta>, Suc p) # s) \<leadsto>\<^sub>h S\<^sub>h h' (v # \<V>) ((\<Delta>, p) # s)"
-| ev\<^sub>h_apply [simp]: "lookup \<C> p = Some Apply\<^sub>b \<Longrightarrow> hlookup h v\<^sub>2 = Lam\<^sub>h \<Delta>' p' \<Longrightarrow>
-    \<C> \<tturnstile> S\<^sub>h h (v\<^sub>1 # v\<^sub>2 # \<V>) ((\<Delta>, Suc p) # s) \<leadsto>\<^sub>h S\<^sub>h h \<V> ((v\<^sub>1 # \<Delta>', p') # (\<Delta>, p) # s)"
+| ev\<^sub>h_apply [simp]: "lookup \<C> p = Some Apply\<^sub>b \<Longrightarrow> hlookup h v\<^sub>2 = Lam\<^sub>h \<Delta>' p' n \<Longrightarrow>
+    \<C> \<tturnstile> S\<^sub>h h (v\<^sub>1 # v\<^sub>2 # \<V>) ((\<Delta>, Suc p) # s) \<leadsto>\<^sub>h S\<^sub>h h \<V> (([v\<^sub>1] # \<Delta>', p') # (\<Delta>, p) # s)"
 | ev\<^sub>h_pushenv [simp]: "lookup \<C> p = Some PushEnv\<^sub>b \<Longrightarrow> 
-    \<C> \<tturnstile> S\<^sub>h h (v # \<V>) ((\<Delta>, Suc p) # s) \<leadsto>\<^sub>h S\<^sub>h h \<V> ((v # \<Delta>, p) # s)"
+    \<C> \<tturnstile> S\<^sub>h h (v # \<V>) ((\<Delta>, Suc p) # s) \<leadsto>\<^sub>h S\<^sub>h h \<V> ((cons_fst v \<Delta>, p) # s)"
 | ev\<^sub>h_return [simp]: "lookup \<C> p = Some Return\<^sub>b \<Longrightarrow> 
     \<C> \<tturnstile> S\<^sub>h h \<V> ((\<Delta>, Suc p) # s) \<leadsto>\<^sub>h S\<^sub>h h \<V> s"
-| ev\<^sub>h_jump [simp]: "lookup \<C> p = Some Jump\<^sub>b \<Longrightarrow> hlookup h v\<^sub>2 = Lam\<^sub>h \<Delta>' p' \<Longrightarrow>
-    \<C> \<tturnstile> S\<^sub>h h (v\<^sub>1 # v\<^sub>2 # \<V>) ((\<Delta>, Suc p) # s) \<leadsto>\<^sub>h S\<^sub>h h \<V> ((v\<^sub>1 # \<Delta>', p') # s)"
+| ev\<^sub>h_jump [simp]: "lookup \<C> p = Some Jump\<^sub>b \<Longrightarrow> hlookup h v\<^sub>2 = Lam\<^sub>h \<Delta>' p' n \<Longrightarrow>
+    \<C> \<tturnstile> S\<^sub>h h (v\<^sub>1 # v\<^sub>2 # \<V>) ((\<Delta>, Suc p) # s) \<leadsto>\<^sub>h S\<^sub>h h \<V> (([v\<^sub>1] # \<Delta>', p') # s)"
 
 theorem determinismh: "\<C> \<tturnstile> \<Sigma> \<leadsto>\<^sub>h \<Sigma>' \<Longrightarrow> \<C> \<tturnstile> \<Sigma> \<leadsto>\<^sub>h \<Sigma>'' \<Longrightarrow> \<Sigma>' = \<Sigma>''"
 proof (induction \<C> \<Sigma> \<Sigma>' rule: eval\<^sub>h.induct)
   case ev\<^sub>h_lookup
-  from ev\<^sub>h_lookup(3, 1, 2) show ?case by (induction rule: eval\<^sub>h.cases) simp_all 
+  from ev\<^sub>h_lookup(4, 1, 2, 3) show ?case by (induction rule: eval\<^sub>h.cases) simp_all 
 next
   case ev\<^sub>h_pushcon
   from ev\<^sub>h_pushcon(3, 1, 2) show ?case by (induction rule: eval\<^sub>h.cases) simp_all 
